veric/SeparationLogicSoundness.v
@@ -14,6 +14,7 @@ Require Import veric.Clight_new.
 Require Import sepcomp.extspec.
 Require Import sepcomp.step_lemmas.
 Require Import veric.juicy_extspec.
+Require Import veric.tycontext.
 Require Import veric.expr.
 Require Import veric.semax.
 Require Import veric.semax_lemmas.
@@ -41,12 +42,12 @@ Axiom semax_prog_rule :
      @semax_prog Espec prog V G ->
      Genv.init_mem prog = Some m ->
      exists b, exists q, 
-       Genv.find_symbol (Genv.globalenv prog) (prog_main prog) = Some b /\
+       Genv.find_symbol (globalenv prog) (prog_main prog) = Some b /\
        core_semantics.initial_core (juicy_core_sem cl_core_sem)
-                    (Genv.globalenv prog) (Vptr b Int.zero) nil = Some q /\
+                    (globalenv prog) (Vptr b Int.zero) nil = Some q /\
        forall n, exists jm, 
        m_dry jm = m /\ level jm = n /\ 
-       jsafeN (@OK_spec Espec) (Genv.globalenv prog) n z q jm.
+       jsafeN (@OK_spec Espec) (globalenv prog) n z q jm.
 
 End SEPARATION_LOGIC_SOUNDNESS.
 
